cp debugging an issue

examples/layeredeffects/RST.Effect.Test.fst
@@ -35,6 +35,19 @@ open RST.Effect
   -LowStar \
   -FStar.ModifiesGen'"
 
+
+assume val rst_get (r:resource)
+: RST (rmem r)
+  r (fun _ -> r)
+  (fun _ -> True)
+  (fun h0 r h1 -> r == h0 /\ h1 == h0)
+
+#set-options "--debug RST.Effect.Test --debug_level Extreme --ugly --print_effect_args --print_implicits --debug_level Rel --debug_level TwoPhases --debug_level LayeredEffects"
+let test (r:resource) : RST unit r (fun _ -> r) (fun _ -> True) (fun _ _ _ -> True) =
+  let r_tmp = r in
+  let h0 = rst_get r_tmp in
+  assert (h0 == h0)
+
 // (*
 // //  * This code doesn't typecheck without the <: Tot nat ascription
 // //  * What happens is:
@@ -141,204 +154,198 @@ open RST.Effect
  
 (*** chacha20 ***)
 
-/// The effect definitions and `rst_frame` are as defined in `examples/layered_effect/RST.Effect.fst`
+// /// The effect definitions and `rst_frame` are as defined in `examples/layered_effect/RST.Effect.fst`
 
-module U32 = FStar.UInt32
+// module U32 = FStar.UInt32
 
-assume val array (a:Type0) : Type0
-assume val length (#a:Type0) (b:array a) : nat
-assume val array_resource (#a:Type0) (b:array a) : resource
-assume val as_rseq (#a:Type0) (b:array a) (#r:resource{array_resource b `is_subresource_of` r}) (h:rmem r)
-: GTot (s:Seq.seq a{Seq.length s == length b})
+// assume val array (a:Type0) : Type0
+// assume val length (#a:Type0) (b:array a) : nat
+// assume val array_resource (#a:Type0) (b:array a) : resource
+// assume val as_rseq (#a:Type0) (b:array a) (#r:resource{array_resource b `is_subresource_of` r}) (h:rmem r)
+// : GTot (s:Seq.seq a{Seq.length s == length b})
 
-assume val index (#a:Type0) (b:array a) (i:U32.t{U32.v i < length b})
-: unit ->
-  RST a
-  (array_resource b)
-  (fun _ -> array_resource b)
-  (fun _ -> True)
-  (fun h0 x h1 ->
-    x == Seq.index (as_rseq b h0) (U32.v i) /\
-    h0 == h1)
+// assume val index (#a:Type0) (b:array a) (i:U32.t{U32.v i < length b})
+// : unit ->
+//   RST a
+//   (array_resource b)
+//   (fun _ -> array_resource b)
+//   (fun _ -> True)
+//   (fun h0 x h1 ->
+//     x == Seq.index (as_rseq b h0) (U32.v i) /\
+//     h0 == h1)
 
-assume val upd (#a:Type0) (b:array a) (i:U32.t{U32.v i < length b}) (v:a)
-: unit ->
-  RST unit
-  (array_resource b)
-  (fun _ -> array_resource b)
-  (fun _ -> True)
-  (fun h0 _ h1 ->
-    let s0 = as_rseq b h0 in
-    let s1 = as_rseq b h1 in
-    Seq.index s1 (U32.v i) == v /\
-    (forall (j:nat).{:pattern Seq.index s1 j} (j < Seq.length s1 /\ j =!= (U32.v i)) ==>
-              (Seq.index s1 j == Seq.index s0 j)))
-
-
-type state = b:array U32.t{length b == 16}
-
-assume val rst_get (r:resource)
-: RST (rmem r)
-  r (fun _ -> r)
-  (fun _ -> True)
-  (fun h0 r h1 -> r == h0 /\ h1 == h0)
+// assume val upd (#a:Type0) (b:array a) (i:U32.t{U32.v i < length b}) (v:a)
+// : unit ->
+//   RST unit
+//   (array_resource b)
+//   (fun _ -> array_resource b)
+//   (fun _ -> True)
+//   (fun h0 _ h1 ->
+//     let s0 = as_rseq b h0 in
+//     let s1 = as_rseq b h1 in
+//     Seq.index s1 (U32.v i) == v /\
+//     (forall (j:nat).{:pattern Seq.index s1 j} (j < Seq.length s1 /\ j =!= (U32.v i)) ==>
+//               (Seq.index s1 j == Seq.index s0 j)))
 
 
-/// `focus_rmem` doesn't work well for me, so adding lemmas that I need for chacha20 function below
-
-assume val as_rseq_focus_rmem1 (#a:Type0)
-  (b1 b2:array a) (h:rmem (array_resource b1 <*> array_resource b2))
-: Lemma (as_rseq b1 h == as_rseq b1 (focus_rmem h (array_resource b1)))
-        [SMTPat (as_rseq b1 h)]
-
-assume val as_rseq_focus_rmem2 (#a:Type0)
-  (b1 b2:array a) (h:rmem (array_resource b1 <*> array_resource b2))
-: Lemma (as_rseq b2 h == as_rseq b2 (focus_rmem h (array_resource b2)))
-        [SMTPat (as_rseq b2 h)]
-
-assume val as_rseq_focus_rmem_inv1 (#a:Type0)
-  (b1 b2:array a) (h0 h1:rmem (array_resource b1 <*> array_resource b2))
-: Lemma
-  (requires focus_rmem h0 (array_resource b1) == focus_rmem h1 (array_resource b1))
-  (ensures as_rseq b1 h0 == as_rseq b1 h1)
-  [SMTPat (focus_rmem h0 (array_resource b1)); SMTPat (focus_rmem h1 (array_resource b1))]
-
-assume val as_rseq_focus_rmem_inv2 (#a:Type0)
-  (b1 b2:array a) (h0 h1:rmem (array_resource b1 <*> array_resource b2))
-: Lemma
-  (requires focus_rmem h0 (array_resource b2) == focus_rmem h1 (array_resource b2))
-  (ensures as_rseq b2 h0 == as_rseq b2 h1)
-  [SMTPat (focus_rmem h0 (array_resource b2)); SMTPat (focus_rmem h1 (array_resource b2))]
+// type state = b:array U32.t{length b == 16}
 
 
-/// `copy_state`
+// /// `focus_rmem` doesn't work well for me, so adding lemmas that I need for chacha20 function below
 
-#set-options "--max_fuel 0 --max_ifuel 0"
-let copy_state
-  (st:state)
-  (ost:state)
-: RST unit
-  (array_resource st <*> array_resource ost)
-  (fun _ -> array_resource st <*> array_resource ost)
-  (fun _ -> True)
-  (fun h0 _ h1 ->
-    focus_rmem h0 (array_resource ost) == focus_rmem h1 (array_resource ost) /\
-    as_rseq st h1 `Seq.equal` as_rseq ost h0)
-= let both_st = array_resource st <*> array_resource ost in
-  let h0 = rst_get both_st in
-  let v =
-    rst_frame both_st (fun _ -> both_st) (array_resource st)
-    (index ost 0ul) in
+// assume val as_rseq_focus_rmem1 (#a:Type0)
+//   (b1 b2:array a) (h:rmem (array_resource b1 <*> array_resource b2))
+// : Lemma (as_rseq b1 h == as_rseq b1 (focus_rmem h (array_resource b1)))
+//         [SMTPat (as_rseq b1 h)]
 
-  rst_frame both_st (fun _ -> both_st) (array_resource ost)
-    (upd st 0ul v);
+// assume val as_rseq_focus_rmem2 (#a:Type0)
+//   (b1 b2:array a) (h:rmem (array_resource b1 <*> array_resource b2))
+// : Lemma (as_rseq b2 h == as_rseq b2 (focus_rmem h (array_resource b2)))
+//         [SMTPat (as_rseq b2 h)]
 
-  let v =
-    rst_frame both_st (fun _ -> both_st) (array_resource st)
-    (index ost 1ul) in
+// assume val as_rseq_focus_rmem_inv1 (#a:Type0)
+//   (b1 b2:array a) (h0 h1:rmem (array_resource b1 <*> array_resource b2))
+// : Lemma
+//   (requires focus_rmem h0 (array_resource b1) == focus_rmem h1 (array_resource b1))
+//   (ensures as_rseq b1 h0 == as_rseq b1 h1)
+//   [SMTPat (focus_rmem h0 (array_resource b1)); SMTPat (focus_rmem h1 (array_resource b1))]
 
-  rst_frame both_st (fun _ -> both_st) (array_resource ost)
-    (upd st 1ul v);
+// assume val as_rseq_focus_rmem_inv2 (#a:Type0)
+//   (b1 b2:array a) (h0 h1:rmem (array_resource b1 <*> array_resource b2))
+// : Lemma
+//   (requires focus_rmem h0 (array_resource b2) == focus_rmem h1 (array_resource b2))
+//   (ensures as_rseq b2 h0 == as_rseq b2 h1)
+//   [SMTPat (focus_rmem h0 (array_resource b2)); SMTPat (focus_rmem h1 (array_resource b2))]
 
-  let v =
-    rst_frame both_st (fun _ -> both_st) (array_resource st)
-    (index ost 2ul) in
 
-  rst_frame both_st (fun _ -> both_st) (array_resource ost)
-    (upd st 2ul v);
+// /// `copy_state`
 
-  let v =
-    rst_frame both_st (fun _ -> both_st) (array_resource st)
-    (index ost 3ul) in
+// #set-options "--max_fuel 0 --max_ifuel 0"
+// let copy_state
+//   (st:state)
+//   (ost:state)
+// : RST unit
+//   (array_resource st <*> array_resource ost)
+//   (fun _ -> array_resource st <*> array_resource ost)
+//   (fun _ -> True)
+//   (fun h0 _ h1 ->
+//     focus_rmem h0 (array_resource ost) == focus_rmem h1 (array_resource ost) /\
+//     as_rseq st h1 `Seq.equal` as_rseq ost h0)
+// = let both_st = array_resource st <*> array_resource ost in
+//   let h0 = rst_get both_st in
+//   let v =
+//     rst_frame both_st (fun _ -> both_st) (array_resource st)
+//     (index ost 0ul) in
 
-  rst_frame both_st (fun _ -> both_st) (array_resource ost)
-    (upd st 3ul v);
+//   rst_frame both_st (fun _ -> both_st) (array_resource ost)
+//     (upd st 0ul v);
 
-  let v =
-    rst_frame both_st (fun _ -> both_st) (array_resource st)
-    (index ost 4ul) in
+//   let v =
+//     rst_frame both_st (fun _ -> both_st) (array_resource st)
+//     (index ost 1ul) in
 
-  rst_frame both_st (fun _ -> both_st) (array_resource ost)
-    (upd st 4ul v);
+//   rst_frame both_st (fun _ -> both_st) (array_resource ost)
+//     (upd st 1ul v);
 
-  let v =
-    rst_frame both_st (fun _ -> both_st) (array_resource st)
-    (index ost 5ul) in
+//   let v =
+//     rst_frame both_st (fun _ -> both_st) (array_resource st)
+//     (index ost 2ul) in
 
-  rst_frame both_st (fun _ -> both_st) (array_resource ost)
-    (upd st 5ul v);
+//   rst_frame both_st (fun _ -> both_st) (array_resource ost)
+//     (upd st 2ul v);
 
-  let v =
-    rst_frame both_st (fun _ -> both_st) (array_resource st)
-    (index ost 6ul) in
+//   let v =
+//     rst_frame both_st (fun _ -> both_st) (array_resource st)
+//     (index ost 3ul) in
 
-  rst_frame both_st (fun _ -> both_st) (array_resource ost)
-    (upd st 6ul v);
+//   rst_frame both_st (fun _ -> both_st) (array_resource ost)
+//     (upd st 3ul v);
 
-  let v =
-    rst_frame both_st (fun _ -> both_st) (array_resource st)
-    (index ost 7ul) in
+//   let v =
+//     rst_frame both_st (fun _ -> both_st) (array_resource st)
+//     (index ost 4ul) in
 
-  rst_frame both_st (fun _ -> both_st) (array_resource ost)
-    (upd st 7ul v);
+//   rst_frame both_st (fun _ -> both_st) (array_resource ost)
+//     (upd st 4ul v);
 
-  let v =
-    rst_frame both_st (fun _ -> both_st) (array_resource st)
-    (index ost 8ul) in
+//   let v =
+//     rst_frame both_st (fun _ -> both_st) (array_resource st)
+//     (index ost 5ul) in
 
-  rst_frame both_st (fun _ -> both_st) (array_resource ost)
-    (upd st 8ul v);
+//   rst_frame both_st (fun _ -> both_st) (array_resource ost)
+//     (upd st 5ul v);
 
-  let v =
-    rst_frame both_st (fun _ -> both_st) (array_resource st)
-    (index ost 9ul) in
+//   let v =
+//     rst_frame both_st (fun _ -> both_st) (array_resource st)
+//     (index ost 6ul) in
 
-  rst_frame both_st (fun _ -> both_st) (array_resource ost)
-    (upd st 9ul v);
+//   rst_frame both_st (fun _ -> both_st) (array_resource ost)
+//     (upd st 6ul v);
 
-  let v =
-    rst_frame both_st (fun _ -> both_st) (array_resource st)
-    (index ost 10ul) in
+//   let v =
+//     rst_frame both_st (fun _ -> both_st) (array_resource st)
+//     (index ost 7ul) in
 
-  rst_frame both_st (fun _ -> both_st) (array_resource ost)
-    (upd st 10ul v);
+//   rst_frame both_st (fun _ -> both_st) (array_resource ost)
+//     (upd st 7ul v);
 
-  let v =
-    rst_frame both_st (fun _ -> both_st) (array_resource st)
-    (index ost 11ul) in
+//   let v =
+//     rst_frame both_st (fun _ -> both_st) (array_resource st)
+//     (index ost 8ul) in
 
-  rst_frame both_st (fun _ -> both_st) (array_resource ost)
-    (upd st 11ul v);
+//   rst_frame both_st (fun _ -> both_st) (array_resource ost)
+//     (upd st 8ul v);
 
-  let v =
-    rst_frame both_st (fun _ -> both_st) (array_resource st)
-    (index ost 12ul) in
+//   let v =
+//     rst_frame both_st (fun _ -> both_st) (array_resource st)
+//     (index ost 9ul) in
 
-  rst_frame both_st (fun _ -> both_st) (array_resource ost)
-    (upd st 12ul v);
+//   rst_frame both_st (fun _ -> both_st) (array_resource ost)
+//     (upd st 9ul v);
 
-  let v =
-    rst_frame both_st (fun _ -> both_st) (array_resource st)
-    (index ost 13ul) in
+//   let v =
+//     rst_frame both_st (fun _ -> both_st) (array_resource st)
+//     (index ost 10ul) in
 
-  rst_frame both_st (fun _ -> both_st) (array_resource ost)
-    (upd st 13ul v);
+//   rst_frame both_st (fun _ -> both_st) (array_resource ost)
+//     (upd st 10ul v);
 
-  let v =
-    rst_frame both_st (fun _ -> both_st) (array_resource st)
-    (index ost 14ul) in
+//   let v =
+//     rst_frame both_st (fun _ -> both_st) (array_resource st)
+//     (index ost 11ul) in
 
-  rst_frame both_st (fun _ -> both_st) (array_resource ost)
-    (upd st 14ul v);
+//   rst_frame both_st (fun _ -> both_st) (array_resource ost)
+//     (upd st 11ul v);
 
-  let v =
-    rst_frame both_st (fun _ -> both_st) (array_resource st)
-    (index ost 15ul) in
+//   let v =
+//     rst_frame both_st (fun _ -> both_st) (array_resource st)
+//     (index ost 12ul) in
 
-  rst_frame both_st (fun _ -> both_st) (array_resource ost)
-    (upd st 15ul v);
+//   rst_frame both_st (fun _ -> both_st) (array_resource ost)
+//     (upd st 12ul v);
 
-  let h1 = rst_get both_st in
+//   let v =
+//     rst_frame both_st (fun _ -> both_st) (array_resource st)
+//     (index ost 13ul) in
 
-  //assert False;
-  Seq.lemma_eq_intro (as_rseq st h1) (as_rseq ost h0)
+//   rst_frame both_st (fun _ -> both_st) (array_resource ost)
+//     (upd st 13ul v);
+
+//   let v =
+//     rst_frame both_st (fun _ -> both_st) (array_resource st)
+//     (index ost 14ul) in
+
+//   rst_frame both_st (fun _ -> both_st) (array_resource ost)
+//     (upd st 14ul v);
+
+//   let v =
+//     rst_frame both_st (fun _ -> both_st) (array_resource st)
+//     (index ost 15ul) in
+
+//   rst_frame both_st (fun _ -> both_st) (array_resource ost)
+//     (upd st 15ul v);
+
+//   let h1 = rst_get both_st in
+
+//   //assert False;
+//   Seq.lemma_eq_intro (as_rseq st h1) (as_rseq ost h0)
